viper-total-heaps/TotalFoldUnfold.thy
@@ -32,7 +32,8 @@ inductive fold_rel :: "'a total_context \<Rightarrow> predicate_ident \<Rightarr
   "\<lbrakk> ViperLang.predicates (program_total ctxt) pred_id = Some pred_decl;
      ViperLang.predicate_decl.body pred_decl = Some pred_body;
      \<omega>0 = \<lparr> get_store_total = nth_option vs, get_trace_total = Map.empty, get_total_full = get_total_full \<omega> \<rparr>;
-     red_exhale ctxt (\<lambda>_. True) \<omega>0 (syntactic_mult (Rep_preal q) pred_body) \<omega>0 (RNormal \<omega>1);
+     red_exhale ctxt (\<lambda>_. True) \<omega>0 (syntactic_mult (Rep_preal q) pred_body) \<omega>0 (RNormal \<omega>1');
+     \<omega>1 = \<omega>\<lparr> get_total_full := get_total_full \<omega>1' \<rparr>;
      get_nm_total_full \<omega>1 + nm_exh = get_nm_total_full \<omega>0;
      \<omega>' = add_to_lpm_total_full \<omega>1 (pred_id,vs) (if q = 0 then None else Some (p2pos q, nm_exh))
    \<rbrakk> \<Longrightarrow>
