viper-total-heaps/TotalStateUtil.thy
@@ -16,6 +16,9 @@ fun get_nm_loc_nm :: "'a nested_mask \<Rightarrow> 'a predicate_loc \<Rightarrow
 fun upd_mh_loc_nm :: "'a nested_mask \<Rightarrow> heap_loc \<Rightarrow> preal \<Rightarrow> 'a nested_mask"
   where "upd_mh_loc_nm nm l p = upd_mh_nm nm ((get_mh_nm nm)( l := p ))"
 
+fun dec_mh_loc_nm :: "'a nested_mask \<Rightarrow> heap_loc \<Rightarrow> preal \<Rightarrow> 'a nested_mask"
+  where "dec_mh_loc_nm (NM mh fnm) l p = NM (mh( l := mh l - p )) fnm"
+
 fun add_to_lpm_nonzero_nm :: "'a nested_mask \<Rightarrow> 'a predicate_loc \<Rightarrow> posreal \<Rightarrow> 'a nested_mask \<Rightarrow> 'a nested_mask"
   where "add_to_lpm_nonzero_nm nm lp p nm' = upd_fnm_nm nm ((get_fnm_nm nm)( lp :=
            Some (option_fold (\<lambda>lpm. (fst lpm + p, snd lpm + nm')) (p, nm') (get_fnm_nm nm lp)) ))"
@@ -39,9 +42,6 @@ fun upd_nm_loc_opt_nm :: "'a nested_mask \<Rightarrow> 'a predicate_loc \<Righta
 
 fun inc_mp_loc_nm :: "'a nested_mask \<Rightarrow> 'a predicate_loc \<Rightarrow> preal \<Rightarrow> 'a nested_mask"
   where "inc_mp_loc_nm (NM mh mp fnm) lp p = NM mh (mp( lp := mp lp + p )) fnm"
-
-fun dec_mh_loc_nm :: "'a nested_mask \<Rightarrow> heap_loc \<Rightarrow> preal \<Rightarrow> 'a nested_mask"
-  where "dec_mh_loc_nm (NM mh mp fnm) l p = NM (mh( l := mh l - p )) mp fnm"
 
 fun dec_mp_loc_nm :: "'a nested_mask \<Rightarrow> 'a predicate_loc \<Rightarrow> preal \<Rightarrow> 'a nested_mask"
   where "dec_mp_loc_nm (NM mh mp fnm) lp p = NM mh (mp( lp := mp lp - p )) fnm"
@@ -68,14 +68,6 @@ fun get_mp_total :: "('a, 'b) total_state_scheme \<Rightarrow> 'a predicate_mask
 fun get_fnm_total :: "('a, 'b) total_state_scheme \<Rightarrow> 'a predicate_nm_fun"
   where "get_fnm_total \<phi> = get_fnm_nm (get_nm_total \<phi>)"
 
-(*
-fun get_m_total :: "('a, 'b) total_state_scheme \<Rightarrow> field_mask \<times> 'a predicate_mask"
-  where "get_m_total \<omega> = (get_mh_total \<omega>, get_mp_total \<omega>)"
-
-fun get_nm_loc_total :: "('a, 'b) total_state_scheme \<Rightarrow> 'a predicate_loc \<Rightarrow> 'a nested_mask option"
-  where "get_nm_loc_total \<phi> lp = get_fnm_total \<phi> lp"
-*)
-
 fun upd_hh_total :: "('a, 'b) total_state_scheme \<Rightarrow> 'a total_heap \<Rightarrow> ('a, 'b) total_state_scheme"
   where "upd_hh_total \<omega> hh = \<omega>\<lparr> get_hh_total := hh \<rparr>"
 
@@ -88,7 +80,31 @@ fun upd_mh_total :: "('a, 'b) total_state_scheme \<Rightarrow> field_mask \<Righ
 fun upd_mh_loc_total :: "('a, 'b) total_state_scheme \<Rightarrow> heap_loc \<Rightarrow> preal \<Rightarrow> ('a, 'b) total_state_scheme"
   where "upd_mh_loc_total \<phi> l p = \<phi>\<lparr> get_nm_total := upd_mh_loc_nm (get_nm_total \<phi>) l p \<rparr>"
 
+fun upd_nm_total :: "('a, 'b) total_state_scheme \<Rightarrow> 'a nested_mask \<Rightarrow> ('a, 'b) total_state_scheme"
+  where "upd_nm_total \<phi> nm = \<phi>\<lparr> get_nm_total := nm \<rparr>"
+
+fun dec_mh_loc_total :: "('a, 'b) total_state_scheme \<Rightarrow> heap_loc \<Rightarrow> preal \<Rightarrow> ('a, 'b) total_state_scheme"
+  where "dec_mh_loc_total \<phi> l p = \<phi>\<lparr> get_nm_total := dec_mh_loc_nm (get_nm_total \<phi>) l p \<rparr>"
+
+fun add_to_nm_total :: "('a, 'b) total_state_scheme \<Rightarrow> 'a nested_mask \<Rightarrow> ('a, 'b) total_state_scheme"
+  where "add_to_nm_total \<phi> nm = \<phi>\<lparr> get_nm_total := get_nm_total \<phi> + nm \<rparr>"
+
+fun mult_nm_total :: "('a, 'b) total_state_scheme \<Rightarrow> preal \<Rightarrow> ('a, 'b) total_state_scheme"
+  where "mult_nm_total \<phi> p = \<phi>\<lparr> get_nm_total := p *\<^sub>s get_nm_total \<phi> \<rparr>"
+
+fun add_to_lpm_total :: "('a, 'b) total_state_scheme \<Rightarrow> 'a predicate_loc \<Rightarrow> posreal \<Rightarrow> 'a nested_mask \<Rightarrow> ('a, 'b) total_state_scheme"
+  where "add_to_lpm_total \<phi> lp p nm' = upd_nm_total \<phi> (add_to_lpm_nonzero_nm (get_nm_total \<phi>) lp p nm')"
+
+fun rm_from_lpm_total :: "('a, 'b) total_state_scheme \<Rightarrow> 'a predicate_loc \<Rightarrow> preal \<Rightarrow> ('a, 'b) total_state_scheme"
+  where "rm_from_lpm_total \<phi> lp p = upd_nm_total \<phi> (rm_from_lpm_nm (get_nm_total \<phi>) lp p)"
+
 (*
+fun get_m_total :: "('a, 'b) total_state_scheme \<Rightarrow> field_mask \<times> 'a predicate_mask"
+  where "get_m_total \<omega> = (get_mh_total \<omega>, get_mp_total \<omega>)"
+
+fun get_nm_loc_total :: "('a, 'b) total_state_scheme \<Rightarrow> 'a predicate_loc \<Rightarrow> 'a nested_mask option"
+  where "get_nm_loc_total \<phi> lp = get_fnm_total \<phi> lp"
+
 fun upd_mp_total :: "('a, 'b) total_state_scheme \<Rightarrow> 'a predicate_mask \<Rightarrow> ('a, 'b) total_state_scheme"
   where "upd_mp_total \<phi> mp = \<phi>\<lparr> get_nm_total := upd_mp_nm (get_nm_total \<phi>) mp \<rparr>"
 
@@ -100,52 +116,28 @@ fun upd_m_total :: "('a, 'b) total_state_scheme \<Rightarrow> field_mask \<times
 
 fun upd_fnm_total :: "('a, 'b) total_state_scheme \<Rightarrow> ('a predicate_loc \<rightharpoonup> 'a nested_mask) \<Rightarrow> ('a, 'b) total_state_scheme"
   where "upd_fnm_total \<phi> fnm = \<phi>\<lparr> get_nm_total := upd_fnm_nm (get_nm_total \<phi>) fnm \<rparr>"
-*)
 
-fun upd_nm_total :: "('a, 'b) total_state_scheme \<Rightarrow> 'a nested_mask \<Rightarrow> ('a, 'b) total_state_scheme"
-  where "upd_nm_total \<phi> nm = \<phi>\<lparr> get_nm_total := nm \<rparr>"
-
-(*
 fun upd_nm_loc_total :: "('a, 'b) total_state_scheme \<Rightarrow> 'a predicate_loc \<Rightarrow> 'a nested_mask \<Rightarrow> ('a, 'b) total_state_scheme"
   where "upd_nm_loc_total \<phi> lp nm = \<phi>\<lparr> get_nm_total := upd_nm_loc_nm (get_nm_total \<phi>) lp nm \<rparr>"
 
 fun upd_nm_loc_opt_total :: "('a, 'b) total_state_scheme \<Rightarrow> 'a predicate_loc \<Rightarrow> 'a nested_mask option \<Rightarrow> ('a, 'b) total_state_scheme"
   where "upd_nm_loc_opt_total \<phi> lp nm = \<phi>\<lparr> get_nm_total := upd_nm_loc_opt_nm (get_nm_total \<phi>) lp nm \<rparr>"
-*)
 
-fun add_to_nm_total :: "('a, 'b) total_state_scheme \<Rightarrow> 'a nested_mask \<Rightarrow> ('a, 'b) total_state_scheme"
-  where "add_to_nm_total \<phi> nm = \<phi>\<lparr> get_nm_total := get_nm_total \<phi> + nm \<rparr>"
-
-(*
 fun add_to_nm_loc_total :: "('a, 'b) total_state_scheme \<Rightarrow> 'a predicate_loc \<Rightarrow> 'a nested_mask \<Rightarrow> ('a, 'b) total_state_scheme"
   where "add_to_nm_loc_total \<phi> lp nm = \<phi>\<lparr> get_nm_total := add_to_nm_loc_nm (get_nm_total \<phi>) lp nm \<rparr>"
 
 fun inc_mp_loc_total :: "('a, 'b) total_state_scheme \<Rightarrow> 'a predicate_loc \<Rightarrow> preal \<Rightarrow> ('a, 'b) total_state_scheme"
   where "inc_mp_loc_total \<phi> lp p = \<phi>\<lparr> get_nm_total := inc_mp_loc_nm (get_nm_total \<phi>) lp p \<rparr>"
 
-fun dec_mh_loc_total :: "('a, 'b) total_state_scheme \<Rightarrow> heap_loc \<Rightarrow> preal \<Rightarrow> ('a, 'b) total_state_scheme"
-  where "dec_mh_loc_total \<phi> l p = \<phi>\<lparr> get_nm_total := dec_mh_loc_nm (get_nm_total \<phi>) l p \<rparr>"
-
 fun dec_mp_loc_total :: "('a, 'b) total_state_scheme \<Rightarrow> 'a predicate_loc \<Rightarrow> preal \<Rightarrow> ('a, 'b) total_state_scheme"
   where "dec_mp_loc_total \<phi> lp p = \<phi>\<lparr> get_nm_total := dec_mp_loc_nm (get_nm_total \<phi>) lp p \<rparr>"
-*)
 
-fun mult_nm_total :: "('a, 'b) total_state_scheme \<Rightarrow> preal \<Rightarrow> ('a, 'b) total_state_scheme"
-  where "mult_nm_total \<phi> p = \<phi>\<lparr> get_nm_total := p *\<^sub>s get_nm_total \<phi> \<rparr>"
-
-(*
 fun mult_nm_loc_total :: "('a, 'b) total_state_scheme \<Rightarrow> 'a predicate_loc \<Rightarrow> preal \<Rightarrow> ('a, 'b) total_state_scheme"
   where "mult_nm_loc_total \<phi> lp p = \<phi>\<lparr> get_nm_total := mult_nm_loc_nm (get_nm_total \<phi>) lp p \<rparr>"
 
 fun mult_rm_nm_loc_total :: "('a, 'b) total_state_scheme \<Rightarrow> 'a predicate_loc \<Rightarrow> preal \<Rightarrow> ('a, 'b) total_state_scheme"
   where "mult_rm_nm_loc_total \<phi> lp p = \<phi>\<lparr> get_nm_total := mult_rm_nm_loc_nm (get_nm_total \<phi>) lp p \<rparr>"
 *)
-
-fun add_to_lpm_total :: "('a, 'b) total_state_scheme \<Rightarrow> 'a predicate_loc \<Rightarrow> posreal \<Rightarrow> 'a nested_mask \<Rightarrow> ('a, 'b) total_state_scheme"
-  where "add_to_lpm_total \<phi> lp p nm' = upd_nm_total \<phi> (add_to_lpm_nonzero_nm (get_nm_total \<phi>) lp p nm')"
-
-fun rm_from_lpm_total :: "('a, 'b) total_state_scheme \<Rightarrow> 'a predicate_loc \<Rightarrow> preal \<Rightarrow> ('a, 'b) total_state_scheme"
-  where "rm_from_lpm_total \<phi> lp p = upd_nm_total \<phi> (rm_from_lpm_nm (get_nm_total \<phi>) lp p)"
 
 
 subsection \<open>Full Total State Getters and Setters\<close>
@@ -162,17 +154,6 @@ fun get_mh_total_full :: "('a, 'b) full_total_state_scheme \<Rightarrow> field_m
 fun get_mp_total_full :: "('a, 'b) full_total_state_scheme \<Rightarrow> 'a predicate_mask"
   where "get_mp_total_full \<omega> = get_mp_total (get_total_full \<omega>)"
 
-(*
-fun get_fnm_total_full :: "('a, 'b) full_total_state_scheme \<Rightarrow> ('a predicate_loc \<rightharpoonup> 'a nested_mask)"
-  where "get_fnm_total_full \<omega> = get_fnm_total (get_total_full \<omega>)"
-
-fun get_nm_loc_total_full :: "('a, 'b) full_total_state_scheme \<Rightarrow> 'a predicate_loc \<Rightarrow> 'a nested_mask option"
-  where "get_nm_loc_total_full \<omega> lp = get_nm_loc_total (get_total_full \<omega>) lp"
-
-fun get_m_total_full :: "('a, 'b) full_total_state_scheme \<Rightarrow> field_mask \<times> 'a predicate_mask"
-  where "get_m_total_full \<omega> = (get_mh_total_full \<omega>, get_mp_total_full \<omega>)"
-*)
-
 fun upd_hh_total_full ::  "('a, 'b) full_total_state_scheme \<Rightarrow> 'a total_heap \<Rightarrow> ('a, 'b) full_total_state_scheme"
   where "upd_hh_total_full \<omega> hh = \<omega>\<lparr> get_total_full := upd_hh_total (get_total_full \<omega>) hh \<rparr>"
 
@@ -180,75 +161,26 @@ fun upd_hh_loc_total_full :: "('a, 'b) full_total_state_scheme \<Rightarrow> hea
   where "upd_hh_loc_total_full \<omega> l v =
         \<omega>\<lparr> get_total_full := upd_hh_loc_total (get_total_full \<omega>) l v \<rparr>"
 
-(*
-fun upd_m_total_full :: "('a, 'b) full_total_state_scheme \<Rightarrow> field_mask \<Rightarrow> 'a predicate_mask \<Rightarrow> ('a, 'b) full_total_state_scheme"
-  where "upd_m_total_full \<omega> m pm = \<omega>\<lparr> get_total_full := upd_mp_total (upd_mh_total (get_total_full \<omega>) m) pm \<rparr>"
-*)
-
 fun upd_mh_total_full :: "('a, 'b) full_total_state_scheme \<Rightarrow> field_mask \<Rightarrow> ('a, 'b) full_total_state_scheme"
   where "upd_mh_total_full \<omega> mh = \<omega>\<lparr> get_total_full :=  upd_mh_total (get_total_full \<omega>) mh \<rparr>"
-
-(*
-fun upd_mp_total_full :: "('a, 'b) full_total_state_scheme \<Rightarrow> 'a predicate_mask \<Rightarrow> ('a, 'b) full_total_state_scheme"
-  where "upd_mp_total_full \<omega> mp = \<omega>\<lparr> get_total_full := upd_mp_total (get_total_full \<omega>) mp \<rparr>"
-*)
 
 fun upd_mh_loc_total_full :: "('a, 'b) full_total_state_scheme \<Rightarrow> heap_loc \<Rightarrow> preal \<Rightarrow> ('a, 'b) full_total_state_scheme"
   where "upd_mh_loc_total_full \<omega> l p =
         \<omega>\<lparr> get_total_full := upd_mh_loc_total (get_total_full \<omega>) l p \<rparr>"
 
-(*
-fun upd_mp_loc_total_full :: "('a, 'b) full_total_state_scheme \<Rightarrow> 'a predicate_loc \<Rightarrow> preal \<Rightarrow> ('a, 'b) full_total_state_scheme"
-  where "upd_mp_loc_total_full \<omega> lp p =
-        \<omega>\<lparr> get_total_full := upd_mp_loc_total (get_total_full \<omega>) lp p \<rparr>"
-
-fun upd_fnm_total_full :: "('a, 'b) full_total_state_scheme \<Rightarrow> ('a predicate_loc \<rightharpoonup> 'a nested_mask) \<Rightarrow> ('a, 'b) full_total_state_scheme"
-  where "upd_fnm_total_full \<omega> fnm = \<omega>\<lparr> get_total_full := upd_fnm_total (get_total_full \<omega>) fnm \<rparr>"
-*)
-
 fun upd_nm_total_full :: "('a, 'b) full_total_state_scheme \<Rightarrow> 'a nested_mask \<Rightarrow> ('a, 'b) full_total_state_scheme"
   where "upd_nm_total_full \<omega> nm = \<omega>\<lparr> get_total_full := (get_total_full \<omega>)\<lparr> get_nm_total := nm \<rparr> \<rparr>"
-
-(*
-fun upd_nm_loc_total_full :: "('a, 'b) full_total_state_scheme \<Rightarrow> 'a predicate_loc \<Rightarrow> 'a nested_mask \<Rightarrow> ('a, 'b) full_total_state_scheme"
-  where "upd_nm_loc_total_full \<omega> lp nm = \<omega>\<lparr> get_total_full := upd_nm_loc_total (get_total_full \<omega>) lp nm \<rparr>"
-
-fun upd_nm_loc_opt_total_full :: "('a, 'b) full_total_state_scheme \<Rightarrow> 'a predicate_loc \<Rightarrow> 'a nested_mask option \<Rightarrow> ('a, 'b) full_total_state_scheme"
-  where "upd_nm_loc_opt_total_full \<omega> lp nm = \<omega>\<lparr> get_total_full := upd_nm_loc_opt_total (get_total_full \<omega>) lp nm \<rparr>"
-*)
-
-fun add_to_nm_total_full :: "('a, 'b) full_total_state_scheme \<Rightarrow> 'a nested_mask \<Rightarrow> ('a, 'b) full_total_state_scheme"
-  where "add_to_nm_total_full \<omega> nm =
-        \<omega>\<lparr> get_total_full := add_to_nm_total (get_total_full \<omega>) nm \<rparr>"
-
-(*
-fun add_to_nm_loc_total_full :: "('a, 'b) full_total_state_scheme \<Rightarrow> 'a predicate_loc \<Rightarrow> 'a nested_mask \<Rightarrow> ('a, 'b) full_total_state_scheme"
-  where "add_to_nm_loc_total_full \<omega> lp nm =
-        \<omega>\<lparr> get_total_full := add_to_nm_loc_total (get_total_full \<omega>) lp nm \<rparr>"
-
-fun inc_mp_loc_total_full :: "('a, 'b) full_total_state_scheme \<Rightarrow> 'a predicate_loc \<Rightarrow> preal \<Rightarrow> ('a, 'b) full_total_state_scheme"
-  where "inc_mp_loc_total_full \<omega> lp p =
-        \<omega>\<lparr> get_total_full := inc_mp_loc_total (get_total_full \<omega>) lp p \<rparr>"
 
 fun dec_mh_loc_total_full :: "('a, 'b) full_total_state_scheme \<Rightarrow> heap_loc \<Rightarrow> preal \<Rightarrow> ('a, 'b) full_total_state_scheme"
   where "dec_mh_loc_total_full \<omega> l p =
         \<omega>\<lparr> get_total_full := dec_mh_loc_total (get_total_full \<omega>) l p \<rparr>"
 
-fun dec_mp_loc_total_full :: "('a, 'b) full_total_state_scheme \<Rightarrow> 'a predicate_loc \<Rightarrow> preal \<Rightarrow> ('a, 'b) full_total_state_scheme"
-  where "dec_mp_loc_total_full \<omega> lp p =
-        \<omega>\<lparr> get_total_full := dec_mp_loc_total (get_total_full \<omega>) lp p \<rparr>"
-*)
+fun add_to_nm_total_full :: "('a, 'b) full_total_state_scheme \<Rightarrow> 'a nested_mask \<Rightarrow> ('a, 'b) full_total_state_scheme"
+  where "add_to_nm_total_full \<omega> nm =
+        \<omega>\<lparr> get_total_full := add_to_nm_total (get_total_full \<omega>) nm \<rparr>"
 
 fun mult_nm_total_full :: "('a, 'b) full_total_state_scheme \<Rightarrow> preal \<Rightarrow> ('a, 'b) full_total_state_scheme"
   where "mult_nm_total_full \<omega> p = \<omega>\<lparr> get_total_full := mult_nm_total (get_total_full \<omega>) p \<rparr>"
-
-(*
-fun mult_nm_loc_total_full :: "('a, 'b) full_total_state_scheme \<Rightarrow> 'a predicate_loc \<Rightarrow> preal \<Rightarrow> ('a, 'b) full_total_state_scheme"
-  where "mult_nm_loc_total_full \<omega> lp p = \<omega>\<lparr> get_total_full := mult_nm_loc_total (get_total_full \<omega>) lp p \<rparr>"
-
-fun mult_rm_nm_loc_total_full :: "('a, 'b) full_total_state_scheme \<Rightarrow> 'a predicate_loc \<Rightarrow> preal \<Rightarrow> ('a, 'b) full_total_state_scheme"
-  where "mult_rm_nm_loc_total_full \<omega> lp p = \<omega>\<lparr> get_total_full := mult_rm_nm_loc_total (get_total_full \<omega>) lp p \<rparr>"
-*)
 
 fun add_to_lpm_nonzero_total_full :: "('a, 'b) full_total_state_scheme \<Rightarrow> 'a predicate_loc \<Rightarrow> posreal \<Rightarrow> 'a nested_mask \<Rightarrow> ('a, 'b) full_total_state_scheme"
   where "add_to_lpm_nonzero_total_full \<omega> lp p nm' = upd_nm_total_full \<omega> (add_to_lpm_nonzero_nm (get_nm_total_full \<omega>) lp p nm')"
@@ -258,6 +190,54 @@ fun add_to_lpm_total_full :: "('a, 'b) full_total_state_scheme \<Rightarrow> 'a 
 
 fun rm_from_lpm_total_full :: "('a, 'b) full_total_state_scheme \<Rightarrow> 'a predicate_loc \<Rightarrow> preal \<Rightarrow> ('a, 'b) full_total_state_scheme"
   where "rm_from_lpm_total_full \<phi> lp p = upd_nm_total_full \<phi> (rm_from_lpm_nm (get_nm_total_full \<phi>) lp p)"
+
+(*
+fun get_fnm_total_full :: "('a, 'b) full_total_state_scheme \<Rightarrow> ('a predicate_loc \<rightharpoonup> 'a nested_mask)"
+  where "get_fnm_total_full \<omega> = get_fnm_total (get_total_full \<omega>)"
+
+fun get_nm_loc_total_full :: "('a, 'b) full_total_state_scheme \<Rightarrow> 'a predicate_loc \<Rightarrow> 'a nested_mask option"
+  where "get_nm_loc_total_full \<omega> lp = get_nm_loc_total (get_total_full \<omega>) lp"
+
+fun get_m_total_full :: "('a, 'b) full_total_state_scheme \<Rightarrow> field_mask \<times> 'a predicate_mask"
+  where "get_m_total_full \<omega> = (get_mh_total_full \<omega>, get_mp_total_full \<omega>)"
+
+fun upd_m_total_full :: "('a, 'b) full_total_state_scheme \<Rightarrow> field_mask \<Rightarrow> 'a predicate_mask \<Rightarrow> ('a, 'b) full_total_state_scheme"
+  where "upd_m_total_full \<omega> m pm = \<omega>\<lparr> get_total_full := upd_mp_total (upd_mh_total (get_total_full \<omega>) m) pm \<rparr>"
+
+fun upd_mp_total_full :: "('a, 'b) full_total_state_scheme \<Rightarrow> 'a predicate_mask \<Rightarrow> ('a, 'b) full_total_state_scheme"
+  where "upd_mp_total_full \<omega> mp = \<omega>\<lparr> get_total_full := upd_mp_total (get_total_full \<omega>) mp \<rparr>"
+
+fun upd_mp_loc_total_full :: "('a, 'b) full_total_state_scheme \<Rightarrow> 'a predicate_loc \<Rightarrow> preal \<Rightarrow> ('a, 'b) full_total_state_scheme"
+  where "upd_mp_loc_total_full \<omega> lp p =
+        \<omega>\<lparr> get_total_full := upd_mp_loc_total (get_total_full \<omega>) lp p \<rparr>"
+
+fun upd_fnm_total_full :: "('a, 'b) full_total_state_scheme \<Rightarrow> ('a predicate_loc \<rightharpoonup> 'a nested_mask) \<Rightarrow> ('a, 'b) full_total_state_scheme"
+  where "upd_fnm_total_full \<omega> fnm = \<omega>\<lparr> get_total_full := upd_fnm_total (get_total_full \<omega>) fnm \<rparr>"
+
+fun upd_nm_loc_total_full :: "('a, 'b) full_total_state_scheme \<Rightarrow> 'a predicate_loc \<Rightarrow> 'a nested_mask \<Rightarrow> ('a, 'b) full_total_state_scheme"
+  where "upd_nm_loc_total_full \<omega> lp nm = \<omega>\<lparr> get_total_full := upd_nm_loc_total (get_total_full \<omega>) lp nm \<rparr>"
+
+fun upd_nm_loc_opt_total_full :: "('a, 'b) full_total_state_scheme \<Rightarrow> 'a predicate_loc \<Rightarrow> 'a nested_mask option \<Rightarrow> ('a, 'b) full_total_state_scheme"
+  where "upd_nm_loc_opt_total_full \<omega> lp nm = \<omega>\<lparr> get_total_full := upd_nm_loc_opt_total (get_total_full \<omega>) lp nm \<rparr>"
+
+fun add_to_nm_loc_total_full :: "('a, 'b) full_total_state_scheme \<Rightarrow> 'a predicate_loc \<Rightarrow> 'a nested_mask \<Rightarrow> ('a, 'b) full_total_state_scheme"
+  where "add_to_nm_loc_total_full \<omega> lp nm =
+        \<omega>\<lparr> get_total_full := add_to_nm_loc_total (get_total_full \<omega>) lp nm \<rparr>"
+
+fun inc_mp_loc_total_full :: "('a, 'b) full_total_state_scheme \<Rightarrow> 'a predicate_loc \<Rightarrow> preal \<Rightarrow> ('a, 'b) full_total_state_scheme"
+  where "inc_mp_loc_total_full \<omega> lp p =
+        \<omega>\<lparr> get_total_full := inc_mp_loc_total (get_total_full \<omega>) lp p \<rparr>"
+
+fun dec_mp_loc_total_full :: "('a, 'b) full_total_state_scheme \<Rightarrow> 'a predicate_loc \<Rightarrow> preal \<Rightarrow> ('a, 'b) full_total_state_scheme"
+  where "dec_mp_loc_total_full \<omega> lp p =
+        \<omega>\<lparr> get_total_full := dec_mp_loc_total (get_total_full \<omega>) lp p \<rparr>"
+
+fun mult_nm_loc_total_full :: "('a, 'b) full_total_state_scheme \<Rightarrow> 'a predicate_loc \<Rightarrow> preal \<Rightarrow> ('a, 'b) full_total_state_scheme"
+  where "mult_nm_loc_total_full \<omega> lp p = \<omega>\<lparr> get_total_full := mult_nm_loc_total (get_total_full \<omega>) lp p \<rparr>"
+
+fun mult_rm_nm_loc_total_full :: "('a, 'b) full_total_state_scheme \<Rightarrow> 'a predicate_loc \<Rightarrow> preal \<Rightarrow> ('a, 'b) full_total_state_scheme"
+  where "mult_rm_nm_loc_total_full \<omega> lp p = \<omega>\<lparr> get_total_full := mult_rm_nm_loc_total (get_total_full \<omega>) lp p \<rparr>"
+*)
 
 
 subsection \<open>Empty States\<close>
